\documentclass[11pt]{article}
\usepackage{fullpage}
\usepackage{amsfonts}
\usepackage{graphicx}

\begin{document}

\begin{center}The Quadratic Equation is defined as:\end{center} 
\begin{Large}$$x = \frac{-b \pm \sqrt{b^2 - 4ac}}{2a}$$\end{Large}


\begin{center} 
	The equation, \begin{Large}$3x^2 + 4x + 3$\end{Large}, \\assuming \begin{Large}$a = 3, b = 4, c = 3$\end{Large}\\ plugged 		into the quadratic equation is:
\end{center}

\begin{Large}$$x = \frac{-(4) \pm \sqrt{(4)^2 - 4(3)(3)}}{2(3)}$$\end{Large}

\begin{center}Simplified, is:\end{center}

\begin{Large}$$x = \frac{-4 \pm \sqrt{16 - 36}}{6}$$\end{Large}

\begin{Large}$$x = \frac{-4 \pm \sqrt{-20}}{6}$$\end{Large}

\begin{Large}$$x = \frac{-4 \pm \sqrt{20}i}{6}$$\end{Large}

\begin{Large}$$x = \frac{-4 \pm 2\sqrt{5}i}{6}$$\end{Large}

\begin{Large}$$x = \frac{-2 \pm \sqrt{5}i}{3}$$\end{Large}

\begin{center}\begin{Large}$x = \displaystyle\frac{1}{3}(-2 + \sqrt{5}i)$ and $x = \displaystyle\frac{1}{3}(-2 - \sqrt{5}i)$\end{Large}\end{center}

\end{document}