%Quadratic Equation calculator to LaTeX v1.0.0

\documentclass[12pt]{article}
\usepackage{fullpage}
\usepackage{amsfonts}
\usepackage{graphicx}

\begin{document}
	\begin{center}
		The Quadratic Equation is defined as:
	\end{center} 
	\begin{Large}
		$$x = \frac{-b \pm \sqrt{b^2 - 4ac}}{2a}$$	
	\end{Large}
	\begin{center} 
		The equation, 
			\begin{Large}
				$3x^2 + 4x + 3$
			\end{Large}, 
		\\assuming
			\begin{Large}
				$a = 3, b = 4, c = 3$
			\end{Large}
		\\ plugged into the quadratic equation is:
	\end{center}
	\begin{Large}
		$$x = \frac{-(4) \pm \sqrt{(4)^2 - 4(3)(3)}}{2(3)}$$
	\end{Large}
	\begin{center}
		Simplified, is:
	\end{center}
	\begin{Large}
		$$x = \frac{-4 \pm \sqrt{16 - 36}}{6}$$
	\end{Large}
	\begin{Large}
		$$x = \frac{-4 \pm \sqrt{-20}}{6}$$
	\end{Large}
	\begin{Large}
		$$x = \frac{-4 \pm \sqrt{20}i}{6}$$
	\end{Large}
	\begin{Large}
		$$x = \frac{-4 \pm 2\sqrt{5}i}{6}$$
	\end{Large}
	\begin{Large}
		$$x = \frac{-2 \pm \sqrt{5}i}{3}$$
	\end{Large}
	\begin{center}
		The roots are:
		\begin{Large}
			$x = \displaystyle\frac{1}{3}(-2 + \sqrt{5}i)$ 
		\end{Large}
		and
		\begin{Large}
			$x = \displaystyle\frac{1}{3}(-2 - \sqrt{5}i)$
		\end{Large}
	\end{center}
\end{document}
